\documentclass[]{panel}

\usepackage[utf8]{inputenc}

\pagenumbering{gobble}
\usepackage{geometry}
 \geometry{
 a4paper,
 left=3cm,
 top=3.15cm,
 }

\usepackage{indentfirst}
\usepackage{amsfonts}


\newcommand{\Items}{Name : Batuhan Karaca, ID : 2310191}
\newcommand{\ItemCount}{2}

\newcommand{\Itemzzz}{The work includes modifications written in LaTex}
\newcommand{\ItemCounT}{1}


\begin{document}

\setPanel{north west}\Items\ItemCount 
\setPanel{south west}\Itemzzz\ItemCounT


\section*{Proof of Memoryless Property of the Exponential Distribution}
Suppose that an Exponential variable $T$ represents waiting time. Memoryless 
property means that the fact of having waited for $t$ minutes gets \textit{“forgotten”} ,
and it does not affect the future waiting time. Regardless of the event $T > t$, 
when the total waiting time exceeds $t$, the remaining waiting time still has 
Exponential distribution with the same parameter.
Mathematically,
\\ \\
\begin{tabular}{l l}
    & $P\{ T>t+x\ |\ T>t \} = P\{ T>x \} $ \\
\end{tabular}
\\ \\
In this formula, $t$ is the already elapsed portion of waiting time, and $x$ is the additional,
remaining time.
\\ \\
\subsection*{PROOF}
We know that the \textit{pdf} of Exponential Distribution
\\ \\
\begin{tabular}{l l}
    & $f(t) = \lambda e^{-\lambda t}$ \\
\end{tabular}
\\ \\
Then the probability
\\ \\
\begin{tabular}{l l l}
    & $P\{ T>x \} $&$= \int_x^\infty f(t)dt$ \\
    &&\\
    &&$ = \int_x^\infty \lambda e^{-\lambda t}dt $ \\
    &&\\
    &&$ = lim_{K \rightarrow \infty} \int_x^K \lambda e^{-\lambda t}dt  $ \\
    &&\\
    &&$ = lim_{K \rightarrow \infty} [-e^{-\lambda t}]_x^K $ \\
    &&\\
    &&$ = lim_{K \rightarrow \infty} (e^{-\lambda x}-e^{-\lambda K} )$ \\
    &&\\
    &&$ = e^{-\lambda x}$ \\
\end{tabular}
\\ \\
Using the formula for the conditional probability
\\ \\
\begin{tabular}{l l l}
    & $P\{ T>t+x\ |\ T>t \} $&$= \frac{P\{ T>t+x\ \cap\ T>t \}}{P\{T>t\}}$ \\
    &&\\
    &&$ = \frac{P\{ T>t+x \}}{P\{T>t\}} $ \\
    &&\\
    &&$ = \frac{e^{-\lambda (t+x)}}{e^{-\lambda t}} $\\
    &&\\
    &&$ = e^{-\lambda x}$ \\
\end{tabular}



\end{document}

